

応用数理解析

No.

Date

氏名: 東田 悠希 ID: 1116191012

演習問題1

1) $f(t) = e^{-\alpha|t|} \quad (\alpha > 0)$

$$f(t) = \begin{cases} e^{-\alpha t} & (t \geq 0) \\ e^{\alpha t} & (t < 0) \end{cases}$$

$$\begin{aligned} F(\omega) &= \int_{-\infty}^0 e^{\alpha t} e^{-i\omega t} dt + \int_0^{\infty} e^{-\alpha t} e^{-i\omega t} dt \\ &= \int_{-\infty}^0 e^{t(\alpha - i\omega)} dt + \int_0^{\infty} e^{t(-\alpha - i\omega)} dt \\ &= \left[\frac{1}{\alpha - i\omega} e^{t(\alpha - i\omega)} \right]_{-\infty}^0 + \left[\frac{1}{-\alpha - i\omega} e^{t(-\alpha - i\omega)} \right]_0^{\infty} \\ &= \frac{1}{\alpha - i\omega} - 0 + 0 - \left(\frac{1}{-\alpha - i\omega} \right) \\ &= \frac{1}{\alpha - i\omega} + \frac{1}{\alpha + i\omega} = \frac{2\alpha}{\alpha^2 + \omega^2} \end{aligned}$$

2) $f(t) = \begin{cases} 1 - \frac{|t|}{T} & (|t| \leq T) \\ 0 & (|t| > T) \end{cases}$

$$\begin{aligned} F(\omega) &= \int_{-\infty}^{\infty} f(t) e^{-i\omega t} dt \\ &= \int_{-T}^{-T} 0 \cdot e^{-i\omega t} dt + \int_{-T}^T \left(1 - \frac{|t|}{T}\right) e^{-i\omega t} dt + \int_T^{\infty} 0 \cdot e^{-i\omega t} dt \\ &= \int_{-T}^T \left(1 - \frac{|t|}{T}\right) e^{-i\omega t} dt = \int_{-T}^0 \left(1 + \frac{t}{T}\right) e^{-i\omega t} dt + \int_0^T \left(1 - \frac{t}{T}\right) e^{-i\omega t} dt \\ &= \int_{-T}^0 \left(e^{-i\omega t} + \frac{t}{T} e^{-i\omega t}\right) dt + \int_0^T \left(e^{-i\omega t} - \frac{t}{T} e^{-i\omega t}\right) dt \\ &= \int_{-T}^0 e^{-i\omega t} dt + \frac{1}{T} \int_{-T}^0 t e^{-i\omega t} dt + \int_0^T e^{-i\omega t} dt - \frac{1}{T} \int_0^T t e^{-i\omega t} dt \\ &= 2 \int_0^T t e^{-i\omega t} dt = -\frac{1}{i\omega} t e^{-i\omega t} + \frac{1}{i\omega} \int e^{-i\omega t} dt \\ &= -\frac{t}{i\omega} e^{-i\omega t} + \frac{1}{\omega^2} e^{-i\omega t} + C \quad (C \text{ は積分定数}) \end{aligned}$$

2'から

$$\begin{aligned} F(\omega) &= \left[-\frac{1}{i\omega} e^{-i\omega t} \right]_{-T}^0 + \frac{1}{T} \left[\frac{t}{i\omega} e^{-i\omega t} + \frac{1}{\omega^2} e^{-i\omega t} \right]_{-T}^0 + \left[-\frac{1}{i\omega} e^{-i\omega t} \right]_0^T \\ &= -\frac{1}{i\omega} (1 - e^{i\omega T}) + \frac{1}{T} \left(\frac{1}{i\omega} - \frac{T e^{i\omega T}}{i\omega} - \frac{1}{\omega^2} e^{i\omega T} \right) - \frac{1}{i\omega} (e^{i\omega T} - 1) \\ &= \frac{1}{i\omega} (e^{i\omega T} - e^{-i\omega T}) + \frac{1}{T} \left\{ \frac{1}{\omega^2} (2 - e^{i\omega T} - e^{-i\omega T}) - \frac{T e^{i\omega T}}{i\omega} + \frac{T e^{-i\omega T}}{i\omega} \right\} \\ &= \frac{2 \sin \omega T}{\omega} + \frac{1}{T} \left\{ \frac{1}{\omega^2} (2 - 2 \cos \omega T) - \frac{T}{\omega} 2 \sin \omega T \right\} \\ &= \frac{2}{\omega^2 T} (1 - \cos \omega T) \end{aligned}$$

$$(3) f(t) = \begin{cases} \sin t & (|t| \leq \pi) \\ 0 & (|t| > \pi) \end{cases}$$

$$F(\omega) = \int_{-\infty}^{\infty} f(t) e^{-i\omega t} dt$$

$$= \int_{-\pi}^{\pi} 0 \times e^{-i\omega t} dt + \int_{-\pi}^{\pi} \sin t e^{-i\omega t} dt + \int_{\pi}^{\infty} 0 \times e^{-i\omega t} dt$$

$$= \int_{-\pi}^{\pi} \sin t \times e^{-i\omega t} dt$$

$$= 2 \int_0^{\pi} \sin t \times e^{-i\omega t} dt = I \text{ 求める}$$

$$I = \int \sin t e^{-i\omega t} dt = -\frac{1}{i\omega} e^{-i\omega t} \sin t + \frac{1}{i\omega} \int e^{-i\omega t} \cos t dt + C$$

$$= -\frac{1}{i\omega} e^{-i\omega t} \sin t + \frac{1}{i\omega} \left\{ -\frac{1}{i\omega} e^{-i\omega t} \cos t + \frac{1}{i\omega} \int e^{-i\omega t} \sin t dt \right\} + C$$

$$= -\frac{1}{i\omega} e^{-i\omega t} \sin t + \frac{1}{\omega^2} e^{-i\omega t} \cos t + \frac{1}{\omega^2} \int e^{-i\omega t} \sin t dt + C$$

$$\left(1 - \frac{1}{\omega^2}\right) I = \frac{e^{-i\omega t}}{\omega} \left(\frac{\cos t}{\omega} + i \sin t \right) \quad (C: \text{積分定数})$$

$$I = \frac{1}{\omega^2 - 1} (\cos t + i \omega \sin t) e^{-i\omega t}$$

5, 2

$$F(\omega) = \int_{-\pi}^{\pi} \sin t \times e^{-i\omega t} dt$$

$$= \frac{1}{\omega^2 - 1} \left[(\cos t + i \omega \sin t) e^{-i\omega t} \right]_{-\pi}^{\pi}$$

$$= \frac{1}{\omega^2 - 1} \{ (-1) e^{-i\omega\pi} - (-1) e^{i\omega\pi} \}$$

$$= \frac{1}{\omega^2 - 1} (-e^{-i\omega\pi} + e^{i\omega\pi})$$

$$= \frac{1}{\omega^2 - 1} (e^{i\omega\pi} - e^{-i\omega\pi})$$

$$= \frac{1}{\omega^2 - 1} \{ \cos \omega\pi + i \sin \omega\pi - \cos(-\omega\pi) - i \sin(-\omega\pi) \}$$

$$= \frac{1}{\omega^2 - 1} \times 2i \sin \omega\pi$$

$$= \frac{2i}{\omega^2 - 1} \sin \omega\pi$$